Monad_Play Around/DNFP/Dutch_National_Flag_Monad_Definitions_Lemmas.thy
@@ -3,7 +3,39 @@ imports
   "Dutch_National_Flag_Monad_Definitions"
 begin
 
+definition sorted_dnfp_pre where
+ "sorted_dnfp_pre e \<equiv> i e = 0
+                    \<and> low e = 0
+                    \<and> high e = length (xs e)"
+
+lemma sorted_dnfp_aux1: "\<lbrakk>sorted_dnfp_pre e\<rbrakk> \<Longrightarrow> low_invariant_is_0_Env e"
+  unfolding sorted_dnfp_pre_def  low_invariant_is_0_Env_def
+  by simp
+
+lemma sorted_dnfp_aux2: "\<lbrakk>sorted_dnfp_pre e\<rbrakk> \<Longrightarrow> invariant_low_to_j_is_1_Env e"
+  unfolding sorted_dnfp_pre_def  invariant_low_to_j_is_1_Env_def
+  by simp
+
+lemma sorted_dnfp_aux3: "\<lbrakk>sorted_dnfp_pre e\<rbrakk> \<Longrightarrow> high_invariant_is_2_Env e"
+  unfolding sorted_dnfp_pre_def  high_invariant_is_2_Env_def
+  by simp
+
+lemma sorted_dnfp: "\<lbrakk>sorted_dnfp_pre e\<rbrakk> \<Longrightarrow> invariants_Env e"
+  unfolding sorted_dnfp_pre_def  invariants_Env_def
+  by (simp add: invariant_low_to_j_is_1_Env_def low_invariant_is_0_Env_def sorted_dnfp_aux3 sorted_dnfp_pre_def)
+
+definition sorted_array :: "env \<Rightarrow> bool" where
+  "sorted_array e \<equiv> invariants_Env e 
+                  \<and> set(xs e) = {0,1,2}
+                  \<and> low e \<le> i e
+                  \<and> i e = high e
+                  \<and> high e \<le> length (xs e)"
+
+lemma sorted_aux: "\<lbrakk>sorted_array e\<rbrakk> \<Longrightarrow> sorted (xs e)"
+  unfolding sorted_array_def invariants_Env_def high_invariant_is_2_Env_def invariant_low_to_j_is_1_Env_def low_invariant_is_0_Env_def
+  by (smt Suc_1 Suc_leD less_le_trans nat_le_linear not_less not_one_le_zero sorted_iff_nth_mono)
   
+
 lemma inc_lowbound_spec: "spec (inc_lowbound_pre e) inc_lowbound (GG (inc_lowbound_post e))"
   unfolding inc_lowbound_pre_def loop_update_action_pre_def GG_def inc_lowbound_post_def loop_update_action_post_def
   apply(simp_all add: inc_lowbound_def)
@@ -258,5 +290,197 @@ definition inc_index_inv :: "env \<Rightarrow> bool" where
 
 lemma inc_index_invariants: "spec inc_index_inv inc_index (GG invariants_Env)"
   by (metis (mono_tags, lifting) GG_def inc_index_inv_def inc_index_invariantBlue inc_index_invariantRed inc_index_invariantWhite invariants_Env_def spec_def split_def)
+
+
+subsection\<open>Loop update action\<close>
+lemma loop_update_action_spec: "spec (loop_update_action_pre_aux e) loop_update_action (GG (loop_update_action_post e))"
+  unfolding loop_update_action_pre_aux_def GG_def loop_update_action_pre_def loop_update_action_post_def
+  apply(simp add: loop_update_action_def)
+  apply (intro get_rule; intro allI; clarify)
+  apply (intro cond_rule)
+  apply(simp add: inc_lowbound_def)
+ apply(intro get_rule; intro allI; simp)
+    apply(intro conj_rule_right)
+       apply (intro seq_rule[of _ _ "(\<lambda>_ y. length (xs e) = length (xs y))"])
+          apply (simp add: spec_def put_def put_state_def swap_def get_state_def xs_Env_def)
+        apply(intro allI; simp)
+        apply(intro get_rule; intro allI)
+       apply (intro seq_rule[of _ _ "(\<lambda>_ y. length (xs e) = length (xs y))"])
+          apply (simp add: spec_def put_def put_state_def swap_def get_state_def i_Env_def)
+         apply(intro allI; simp)
+        apply(intro get_rule; intro allI)
+          apply (simp add: spec_def put_def put_state_def swap_def get_state_def low_Env_def)
+         apply (intro seq_rule[of _ _ "(\<lambda>_ y. high e = high y)"])
+        apply (simp add: spec_def put_def put_state_def swap_def get_state_def xs_Env_def)
+         apply(intro allI; simp)
+        apply(intro get_rule; intro allI)
+         apply (intro seq_rule[of _ _ "(\<lambda>_ y. high e = high y)"])
+          apply (simp add: spec_def put_def put_state_def swap_def get_state_def i_Env_def)
+         apply(intro allI; simp)
+       apply(intro get_rule; intro allI)
+          apply (simp add: spec_def put_def put_state_def swap_def get_state_def low_Env_def)
+      apply (intro seq_rule[of _ _ "(\<lambda>_ y. low e = low y)"])
+          apply (simp add: spec_def put_def put_state_def swap_def get_state_def xs_Env_def i_Env_def)
+        apply(intro allI; simp)
+        apply(intro get_rule; intro allI)
+        apply(intro seq_rule[of _ _ "(\<lambda>_ y. low e = low y)"])
+          apply (simp add: spec_def put_def put_state_def  get_state_def i_Env_def)
+        apply(intro allI; simp)
+        apply(intro get_rule; intro allI)
+      apply(simp add: spec_def put_def get_state_def put_state_def low_Env_def)
+     apply (intro seq_rule[of _ _ "(\<lambda>_ y. i y = i e)"])
+     apply (simp add: spec_def put_def put_state_def swap_def get_state_def xs_Env_def)
+    apply(intro allI; simp)
+    apply(intro get_rule; intro allI)
+     apply (intro seq_rule[of _ _ "(\<lambda>_ y. i y > i e)"])
+      apply (simp add: spec_def put_def put_state_def  get_state_def i_Env_def)
+    apply(intro allI; simp)
+     apply(intro get_rule; intro allI)
+      apply (simp add: spec_def put_def put_state_def  get_state_def low_Env_def)
+   apply (intro seq_rule[of _ _ "(\<lambda>_ y. i y < high y \<and> i y = i e \<and> high y = high e)"])
+    apply (simp add: spec_def put_def put_state_def swap_def get_state_def xs_Env_def)
+   apply(intro allI; simp)
+   apply(intro get_rule; intro allI)
+   apply (intro seq_rule[of _ _ "(\<lambda>_ y. high y - i y < high e - i e)"])
+    apply (simp add: spec_def put_def put_state_def  get_state_def i_Env_def)
+     apply (linarith)
+   apply(intro allI; simp)
+   apply(intro get_rule; intro allI)
+    apply (simp add: spec_def put_def put_state_def  get_state_def low_Env_def)
+    apply(simp add: dec_highbound_def)
+    apply(intro conj_rule_right)
+        apply (intro get_rule; intro allI; simp)
+        apply (intro seq_rule[of _ _ "(\<lambda>_ y. length (xs e) = length (xs y))"])
+         apply (simp add: spec_def put_def get_state_def put_state_def high_Env_def swap_def)
+        apply (rule allI; simp; intro get_rule; rule allI; simp)
+         apply (simp add: spec_def get_def put_def get_state_def put_state_def xs_Env_def swap_def)
+       apply (intro get_rule; intro allI; simp)
+          apply(intro seq_rule[of _ _ "(\<lambda>x y. high y < high e)"]) 
+        apply (simp add: spec_def get_def put_def get_state_def put_state_def high_Env_def)
+      apply (intro allI; simp)
+        apply (intro get_rule; intro allI; simp)
+         apply (simp add: spec_def get_def put_def get_state_def put_state_def xs_Env_def swap_def)
+      apply (intro get_rule; intro allI; simp)
+          apply(intro seq_rule[of _ _ "(\<lambda>x y. low e \<le> low y)"]) 
+        apply (simp add: spec_def get_def put_def get_state_def put_state_def high_Env_def)
+      apply (intro allI; simp)
+      apply (intro get_rule; intro allI; simp)
+         apply (simp add: spec_def get_def put_def get_state_def put_state_def xs_Env_def swap_def)
+      apply (intro get_rule; intro allI; simp)
+          apply(intro seq_rule[of _ _ "(\<lambda>x y. i e \<le> i y)"]) 
+        apply (simp add: spec_def get_def put_def get_state_def put_state_def high_Env_def)
+      apply (intro allI; simp)
+      apply (intro get_rule; intro allI; simp)
+       apply (simp add: spec_def get_def put_def get_state_def put_state_def xs_Env_def swap_def)
+      apply (intro get_rule; intro allI; simp)
+      apply(intro seq_rule[of _ _ "(\<lambda>x y. high y - i y < high e - i e)"]) 
+     apply (simp add: spec_def get_def put_def get_state_def put_state_def high_Env_def)
+  apply(linarith)
+     apply(intro allI; simp)
+    apply (intro get_rule; intro allI; simp)
+    apply (simp add: spec_def get_def put_def get_state_def put_state_def xs_Env_def swap_def)
+    apply(simp add: inc_index_def)
+    apply(intro conj_rule_right)
+    apply (intro get_rule; intro allI; simp)
+    apply (simp add: spec_def get_def put_def get_state_def put_state_def i_Env_def)
+    apply (intro get_rule; intro allI; simp)
+    apply (simp add: spec_def get_def put_def get_state_def put_state_def i_Env_def)
+    apply (intro get_rule; intro allI; simp)
+     apply (simp add: spec_def get_def put_def get_state_def put_state_def i_Env_def)
+    apply (intro get_rule; intro allI; simp)
+    apply (simp add: spec_def get_def put_def get_state_def put_state_def i_Env_def)
+    apply (intro get_rule; intro allI; simp)
+   apply (simp add: spec_def get_def put_def get_state_def put_state_def i_Env_def)
+  by(linarith)
+
+subsubsection\<open>Invariants\<close>
+text\<open>Should I add some more assumptions (The preconditions from the 3 methods inside loop_update_action) here in the precondition?\<close>
+lemma loop_update_action_invariantRed: "spec loop_update_action_inv1 loop_update_action (GG low_invariant_is_0_Env)"
+   unfolding loop_update_action_inv1_def loop_update_action_pre_def  GG_def low_invariant_is_0_Env_def
+  apply(simp add: loop_update_action_def)
+  apply (intro get_rule; intro allI; clarify)
+   apply (intro cond_rule)
+     apply(simp add: inc_lowbound_def)
+     apply (intro get_rule; intro allI; simp)
+  apply(intro seq_rule[of _ _ "(\<lambda>x e. xs e ! low e = 0 \<and>  (\<forall>x<low e. xs e ! x = 0))"])
+      apply (simp add: spec_def put_def put_state_def swap_def get_state_def xs_Env_def)
+   apply auto[1]
+  apply(intro allI; simp)
+  apply(intro get_rule; intro allI)
+  apply(intro seq_rule[of _ _ "(\<lambda>x e. xs e ! low e = 0 \<and> (\<forall>x<low e. xs e ! x = 0))"])
+   apply (simp add: spec_def put_def put_state_def get_state_def i_Env_def)
+  apply(intro allI; simp)
+  apply(intro get_rule; intro allI)
+     apply (simp add: spec_def put_def put_state_def get_state_def low_Env_def)
+   using less_antisym apply blast
+     apply(simp add: dec_highbound_def)
+     apply (intro get_rule; intro allI; simp)
+      apply(intro seq_rule[of _ _ "(\<lambda>x e. (\<forall>x<low e. xs e ! x = 0) \<and> high e \<le> length (xs e) \<and> high e \<ge> i e \<and> low e \<le> i e)"]) 
+       apply (simp add: spec_def get_def put_def get_state_def put_state_def high_Env_def)
+       apply(linarith)
+      apply(intro allI; simp)
+     apply (intro get_rule; intro allI; simp)
+      apply (simp add: spec_def get_def put_def get_state_def put_state_def xs_Env_def swap_def)
+     apply(simp add: inc_index_def)
+     apply (intro get_rule; intro allI; simp)
+   by (simp add: spec_def get_def put_def get_state_def put_state_def i_Env_def)
+
+lemma loop_update_action_invariantWhite: "spec loop_update_action_inv2 loop_update_action (GG invariant_low_to_j_is_1_Env)"
+   unfolding loop_update_action_inv2_def loop_update_action_pre_def  GG_def invariant_low_to_j_is_1_Env_def
+  apply(simp add: loop_update_action_def)
+  apply (intro get_rule; intro allI; clarify)
+   apply (intro cond_rule)
+     apply(simp add: inc_lowbound_def)
+     apply (intro get_rule; intro allI; simp)
+   apply (simp add: spec_def put_def put_state_def  get_state_def xs_Env_def swap_def get_def i_Env_def low_Env_def return_def)
+   apply(intro allI)
+     apply (simp add: nth_list_update)
+     apply(simp add: dec_highbound_def)
+        apply(intro get_rule; intro allI; simp)
+    apply(intro seq_rule[of _ _ "(\<lambda>x e. low e \<le> i e \<and> high e \<ge> i e \<and> length (xs e) > high e \<and> (\<forall>x. low e \<le> x \<and> x < i e \<longrightarrow> xs e ! x = Suc 0))"])
+     apply (simp add: spec_def put_def put_state_def get_state_def high_Env_def swap_def)
+    apply linarith
+     apply(intro allI; simp)
+    apply(intro get_rule;intro allI; simp)
+   apply (simp add: spec_def put_def put_state_def get_state_def xs_Env_def swap_def)
+   apply(simp add: inc_index_def)
+   apply(intro get_rule;intro allI; simp)
+   apply (simp add: spec_def put_def put_state_def get_state_def i_Env_def)
+   apply(intro allI)
+   using nat_neq_iff by fastforce
+
+lemma value_must_be_one : "\<lbrakk>xs e ! i e  \<noteq> 0 ; xs e! i e \<noteq> 2 ; i e < length (xs e) ; set(xs e) \<subseteq> {0,1,2}\<rbrakk> \<Longrightarrow> xs e ! i e = 1"
+  by (smt insertE insert_subset mk_disjoint_insert nth_mem singletonD)
+
+lemma value_must_be_two_aux : "\<lbrakk>xs e ! i e  \<noteq> 0 ; xs e! i e \<noteq> 1 ; i e < length (xs e) ; set(xs e) \<subseteq> {0,1,2}\<rbrakk> \<Longrightarrow> xs e ! i e = 2"
+  by (smt insertE insert_subset mk_disjoint_insert nth_mem singletonD)
+
+lemma value_must_be_two : "\<lbrakk>xs e ! i e  > 0 ; xs e! i e > 1 ; i e < length (xs e) ; set(xs e) \<subseteq> {0,1,2}\<rbrakk> \<Longrightarrow> xs e ! i e = 2"
+  using nat_neq_iff value_must_be_two_aux by blast
+
+lemma loop_update_action_invariantBlue: "spec loop_update_action_inv3 loop_update_action (GG high_invariant_is_2_Env)"
+   unfolding loop_update_action_inv3_def loop_update_action_pre_def  GG_def high_invariant_is_2_Env_def
+  apply(simp add: loop_update_action_def)
+  apply (intro get_rule; intro allI; clarify)
+   apply (intro cond_rule)
+     apply(simp add: inc_lowbound_def) 
+     apply(intro get_rule;intro allI; simp)
+  apply(intro seq_rule[of _ _ "(\<lambda>x e. \<forall>x. x \<ge> high e \<and> x < length (xs e) \<longrightarrow> xs e ! x = 2)"])
+   apply (simp add: spec_def put_def put_state_def swap_def get_state_def xs_Env_def)
+      apply(intro allI; simp)
+  apply(intro get_rule; intro allI)
+  apply(intro seq_rule[of _ _ "(\<lambda>x e. \<forall>x. x \<ge> high e \<and> x < length (xs e) \<longrightarrow> xs e ! x = 2)"])
+   apply (simp add: spec_def put_def put_state_def get_state_def i_Env_def)
+  apply(intro allI; simp)
+  apply(intro get_rule; intro allI)
+     apply (simp add: spec_def put_def put_state_def get_state_def low_Env_def)
+    apply(simp_all add: dec_highbound_def)
+    apply(intro get_rule; intro allI; simp)
+     apply (simp add: spec_def put_def put_state_def get_state_def high_Env_def xs_Env_def swap_def get_def return_def)
+   apply(intro allI)
+   apply (smt One_nat_def Suc_leI Suc_pred le_less length_list_update less_Suc_eq_0_disj less_imp_Suc_add less_le_trans nth_list_update value_must_be_two)
+   apply(simp add: inc_index_def)
+    apply(intro get_rule; intro allI; simp)
+   by (simp add: spec_def put_def put_state_def get_state_def i_Env_def)
 
 end
